@@ -1,1 +1,5 @@
-import Xv6.BioPool
+import Xv6.SpecPanic
+import Xv6.SpecAcquiresleep
+import Xv6.SpecVirtioDiskRw
+open Xv6 in
+#eval (panicSlots, acquiresleepSlots, virtioDiskRwSlots, sleepSlots)
